make_makefile.sh
@@ -1,0 +1,2 @@
+#!/bin/sh
+coq_makefile -R "." FormalSystems -o makefile *v */*v
